src/arch/x64/X64.Vale.Decls_i.fsti
@@ -88,6 +88,7 @@ val va_fuel_default : unit -> va_fuel
 [@va_qattr] unfold let va_op_shift_amt64_reg (r:reg) : va_shift_amt = OReg r
 [@va_qattr] unfold let va_op_cmp_reg (r:reg) : va_cmp = OReg r
 [@va_qattr] unfold let va_const_cmp (n:int) : va_cmp = OConst n
+[@va_qattr] unfold let va_coerce_reg_opr64_to_cmp (r:va_operand_reg_opr64) : va_cmp = r
 [@va_qattr] unfold let va_coerce_register_to_operand (r:va_register) : va_operand = OReg r
 [@va_qattr] unfold let va_coerce_operand_to_reg_operand (o:va_operand{OReg? o}) : va_reg_operand = o
 [@va_qattr] unfold let va_coerce_dst_operand_to_reg_operand (o:va_dst_operand{OReg? o}) : va_reg_operand = o
