src/lib/util/Words.Seq_i.fsti
@@ -30,6 +30,9 @@ val nat_to_four_to_nat (x:four (natN (pow2_norm 8))) :
 val four_to_seq_to_four_LE (#a:Type) (x:seq4 a) :
   Lemma (four_to_seq_LE (seq_to_four_LE x) == x)
 
+val seq_to_four_to_seq_LE (#a:Type) (x:four a) :
+  Lemma (seq_to_four_LE (four_to_seq_LE x) == x)
+
 val four_to_seq_to_four_BE (#a:Type) (x:seq4 a) :
   Lemma (four_to_seq_BE (seq_to_four_BE x) == x)
 
@@ -43,10 +46,16 @@ val seq_nat8_to_seq_nat32_to_seq_nat8_LE (x:seq nat32) :
   Lemma (seq_nat8_to_seq_nat32_LE (seq_nat32_to_seq_nat8_LE x) == x)
   [SMTPat (seq_nat8_to_seq_nat32_LE (seq_nat32_to_seq_nat8_LE x))]
 
-(*
-val seq_four_to_seq_LE_injective: unit ->
-  Lemma (forall (#a:Type) (x x':seq (four a)). seq_four_to_seq_LE x == seq_four_to_seq_LE x' ==> x == x')
+val seq_four_to_seq_LE_injective: (a:eqtype) ->
+  Lemma (forall (x x':seq (four a)). seq_four_to_seq_LE x == seq_four_to_seq_LE x' ==> x == x')
 
+val seq_four_to_seq_LE_injective_specific (#a:eqtype) (x x':seq (four a)) :
+  Lemma (seq_four_to_seq_LE x == seq_four_to_seq_LE x' ==> x == x')
+
+val four_to_seq_LE_injective (a:eqtype) :
+  Lemma (forall (x x': four a) . four_to_seq_LE x == four_to_seq_LE x' ==> x == x')
+
+(*
 val seq_to_seq_four_LE_injective: unit ->
   Lemma (forall (#a:Type) (x:seq a{length x % 4 == 0}) (x':seq a{length x' % 4 == 0}) . seq_to_seq_four_LE x == seq_to_seq_four_LE x' ==> x == x')
 *)
